
\documentclass{article}%
\usepackage{amsmath}
\usepackage{graphicx}
\usepackage{amsfonts}%
\usepackage{amssymb}


\setlength{\topmargin}{-0.75in}
\setlength{\textheight}{9.25in}
\setlength{\oddsidemargin}{0.0in}
\setlength{\evensidemargin}{0.0in}
\setlength{\textwidth}{6.5in}
\def\labelenumi{\arabic{enumi}.}
\def\theenumi{\arabic{enumi}}
\def\labelenumii{(\alph{enumii})}
\def\theenumii{\alph{enumii}}
\def\p@enumii{\theenumi.}
\def\labelenumiii{\arabic{enumiii}.}
\def\theenumiii{\arabic{enumiii}}
\def\p@enumiii{(\theenumi)(\theenumii)}
\def\labelenumiv{\arabic{enumiv}.}
\def\theenumiv{\arabic{enumiv}}
\def\p@enumiv{\p@enumiii.\theenumiii}
\pagestyle{plain}
\setcounter{secnumdepth}{0}
\newtheorem{theorem}{Theorem}
\newtheorem{acknowledgement}[theorem]{Acknowledgement}
\newtheorem{algorithm}[theorem]{Algorithm}
\newtheorem{axiom}[theorem]{Axiom}
\newtheorem{case}[theorem]{Case}
\newtheorem{claim}[theorem]{Claim}
\newtheorem{conclusion}[theorem]{Conclusion}
\newtheorem{condition}[theorem]{Condition}
\newtheorem{conjecture}[theorem]{Conjecture}
\newtheorem{corollary}[theorem]{Corollary}
\newtheorem{criterion}[theorem]{Criterion}
\newtheorem{definition}[theorem]{Definition}
\newtheorem{example}[theorem]{Example}
\newtheorem{exercise}[theorem]{Exercise}
\newtheorem{lemma}[theorem]{Lemma}
\newtheorem{notation}[theorem]{Notation}
\newtheorem{problem}[theorem]{Problem}
\newtheorem{proposition}[theorem]{Proposition}
\newtheorem{remark}[theorem]{Remark}
\newtheorem{solution}[theorem]{Solution}
\newtheorem{summary}[theorem]{Summary}
\newenvironment{proof}[1][Proof]{\textbf{#1.} }{\ \rule{0.5em}{0.5em}}

\newcommand{\lv}{\lVert}
\newcommand{\rv}{\rVert}

\begin{document}

\title{Theoretical Numerical Analysis, Assignment 2}
\author{Chuan Lu}
\date{\today}
\maketitle

\begin{enumerate}

\item Problem 2.4.2

By definition,
\begin{equation}
\begin{aligned}
\lv L_n\rv &= \sup_{v\ne 0}\frac{\lv L_n v\rv}{\lv v\rv}  = \sup_{v \ne 0}\frac{\lv \sum_{i=0}^{n} w_i^{(n)} v(x_i^{(n)}) \rv}{\lv v\rv} \\
&\le \sup_{v \ne 0}\frac{\sum_{i=0}^{n}|w_i^{(n)|}\lv v\rv}{\lv v\rv} \\
&= \sum_{i=0}^{n}\lv |w_i^{(n)}|.
\end{aligned}
\end{equation}
On the other hand, let $v(x) =  1$, then RHS becomes
\begin{equation}
\frac{\lv w_i^{(n)} v\rv}{\lv v\rv} = \sum_{i=0}^{n}|w_i^{(n)}|,
\end{equation}
so
\begin{equation}
\lv L_n\rv = \sum_{i=0}^{n}|w_i^{(n)}|.
\end{equation}

\item Problem 2.4.3

From the textbook we only need to show that 
\begin{equation}
\sup_n \sum_{i=0}^{n}|w_i^{(n)}| < \infty.
\end{equation}

By the assumption,
\begin{equation}
\sup_n \sum_{i=0}^{n}|w_i^{(n)}| = \sup_n \sum_{i=1}^{n}w_i^{(n)} = \sup_n L_n u,
\end{equation}
where $u = u(x) \equiv 1$. Since for all $n$, $u\in \mathbb{P}_{d(n)} $,
\begin{equation}
L_n u = Lu = 1,
\end{equation}
we know $\sup L_n u < \infty $.

\item Problem 2.4.5

First, consider $V = \mathbb{P}[0, 1] $. For a fixed element $v\in \mathbb{P}$, we already know the error of composite trapezoidal rule is
\begin{equation}
E(v) = \frac{1}{12n^3}\sum_{i=0}^{n-1}v''(\xi_i)\le \frac{1}{12n^2}\lv v''\rv.
\end{equation}
Since $\lv v'' \rv < \infty$, we know $E(v) \to 0$ as $n\to\infty$, hence $L_n v \to L_v $.

On the other hand, 
\begin{equation}
\lv L_n\rv = \sum_{i=0}^{n}|w_i^{(n)}| = 1
\end{equation}
for all $n$, so $\sup \lv L_n\rv < \infty $. By Banach-Steinhaus theorem, $L_n v\to Lv $ for all $v\in C[0, 1]$.

\item Problem 2.5.4

By (2.5.5),
\begin{equation}
\ell(v) = (u, v)
\end{equation}
for all $v\in V$. Then let $v = e_j $, we have
\begin{equation}
\ell(e_j) = (u, e_j)
\end{equation}
for all $j$. Then
\begin{equation}
u = \sum_{j=1}^{\infty}(u, e_j)e_j = \sum_{j=1}^{\infty}\ell(e_j)e_j.
\end{equation}

\item Problem 2.7.3

$\Rightarrow$: If $u_n \to u $, then
\begin{equation}
\lim_{n\to\infty} \lv u_n - u\rv = 0,
\end{equation}
so for each $\ell in V'$, 
\begin{equation}
\lim_{n\to\infty}\lv \ell(u_n) - \ell(u)\rv \le\lim_{n\to\infty}\lv \ell\rv \lv u_n-u\rv = 0.
\end{equation}
Then $u_n \rightharpoonup u $. Notice $\lv u_n-u\rv \ge \lv u_n\rv - \lv u\rv $, and $\lv u - u_n\rv \ge \lv u\rv - \lv u_n\rv $ we have
\begin{equation}
\lim_{n\to\infty}\lv u_n\rv - \lv u\rv \le 0, \ \lim_{n\to\infty} \lv u \rv - \lv u_n\rv \le 0.
\end{equation}
Thus $\lv u_n\rv \to \lv u\rv $.

$\Leftarrow$: Consider
\begin{equation}
\lim_{n\to\infty}\lv u_n-u\rv^2 = \lim_{n\to\infty}\lv u_n\rv^2 + \lv u\rv^2 - (u_n, u) - (u, u_n),
\end{equation}
and both $(u, \cdot)$ and $(\cdot, u)$ are linear functionals on $V$, we have
\begin{equation}
\lim_{n\to\infty}\lv u_n - u\rv^2 = \lim_{n\to\infty} \lv u_n\rv^2 + \lv u\rv^2 - \lv u\rv^2 - \lv u\rv^2 = 0.
\end{equation}
Hence $\lv u - u_n\rv \to 0 $.

\end{enumerate}
\end{document}