\documentclass{article}
\usepackage[left=2cm,right=2cm,top=2cm]{geometry}

\usepackage{amsthm,amsmath,amssymb}
\usepackage[numbers]{natbib}
\usepackage{hyperref}
\usepackage{graphicx}
\usepackage{caption}
\usepackage{subcaption}
\newcommand{\bx}{{\mathbf x}}
\newcommand{\ba}{{\mathbf a}}
\newcommand{\bv}{{\mathbf v}}
\newcommand{\bu}{{\mathbf u}}


\newtheorem{theorem}{Theorem}[section]
\newtheorem{proposition}[theorem]{Proposition}
\newtheorem{lemma}[theorem]{Lemma}
\newtheorem{corollary}[theorem]{Corollary}
\newtheorem{remark}{Remark}[section]
\newtheorem{example}[theorem]{Example}


\begin{document}

\title{Management Sciences Topics: Convex Optimization\\ Homework 3}
\date{}
\maketitle

\begin{enumerate}
\item Problem 1

We may change the step size to
$$
\eta_k = \frac{2}{\mu(k+2)}
$$
as when $\mu > 0$ in SSG. Now we show that

First, by three term lemma,
$$
\langle x^{k+1}-x^k, g_x^k\rangle + \frac{1}{2\eta_k}\lVert x^{k+1}-x^k\rVert_2^2 \le \langle x-x^k, g_x^k\rangle + \frac{1}{2\eta_k}\lVert x-x^k\rVert_2^2 - \frac{1}{2\eta_k}\lVert x-x^{k+1}\rVert_2^2.
$$
By strong convexity of $f$ w.r.t. $x$,
$$
f(x^k, y) - f(x^*, y) \le \langle g_x^k, x^k - x^*\rangle - \frac{\mu}{2}\lVert x^k - x^*\rVert_2^2.
$$
Then by mean inequality,
$$
\begin{aligned}
f(x^k, y) - f(x^*, y) &\le \langle x^*-x^k, g_x^k\rangle +\frac{1}{2\eta_k}\lVert x^*-x^k\rVert_2^2-\frac{1}{2\eta_k}\lVert x^*-x^{k+1}\rVert_2^2-\frac{1}{2\eta_k}\lVert x^{k+1}-x^k\rVert_2^2 -\frac{\mu}{2}\lVert x^k-x^*\rVert_2^2 \\
&\le \frac{1}{2}\eta_k \lVert g_x^k\rVert_2^2 + (\frac{1}{2\eta_k}-\frac{\mu}{2})\lVert x^k-x^*\rVert_2^2-\frac{1}{2\eta_k}\lVert x^*-x^{k+1}\rVert_2^2 \\
&\le \frac{1}{2}\eta_k M^2 + (\frac{1}{2\eta_k}-\frac{\mu}{2})\lVert x^k-x^*\rVert_2^2-\frac{1}{2\eta_k}\lVert x^*-x^{k+1}\rVert_2^2 \\
&= \frac{1}{\mu(k+2)}M^2 +\frac{\mu k}{4}\lVert x^k-x^*\rVert_2^2 - \frac{\mu(k+2)}{4}\lVert x^*-x^{k+1}\rVert_2^2.
\end{aligned}
$$
Then
$$
\sum_{k=0}^{K-1}(k+1)(f(x^k, y) - f(x^*, y)) \le \sum_{k=0}^{K-1} \frac{k+1}{\mu(k+2)}M^2 + \sum_{k=0}^{K-1} \frac{\mu k(k+1)}{4}\lVert x^k-x^*\rVert_2^2 - \sum_{k=0}^{K-1} \frac{\mu(k+1)(k+2)}{4}\lVert x^*-x^{k+1}\rVert_2^2,
$$
and
$$
\frac{k(k+1)}{2}(f(\bar{x}, y)-f(x^*, y)) \le \frac{KM^2}{\mu},
$$
so
$$
f(\bar{x}, y)-f(x^*, y) \le \frac{2M^2}{(k+1)\mu}.
$$
Similarly, we have
$$
f(x, \bar{y})-f(x, y^*) \le \frac{2M^2}{(k+1)\mu}.
$$
Lets $y = \bar{y}$ in the first equation and $x = x^* $ in the second equation, by adding these two equations, we get
$$
f(\bar{x}, \bar{y}) - f(x^*, y^*) \le \frac{4M}{(K+1)\mu}.
$$
Then the algorithm has a convergence rate of $O(\frac{1}{k})$.


\item Problem 2.




\end{enumerate}

\end{document}

